update repeat example with wsim

examples/repeat/RepeatIAproof.v
@@ -8,56 +8,40 @@ Set Implicit Arguments.
 Module RepeatIA. Section RepeatIA.
   Import RepeatAS APC APCA.
   Context `{!invG α Σ Γ, !subG Γ Σ, !sinvG Σ Γ α β τ}.
-  Notation iProp := (iProp Σ).
 
-  Variable genv: GEnv.t.
-  Variable u: univ_id.
-  Variable Spc: string → option fspec.
-  Variable SpcPure: string → option fspec.
-  Variable SpcPureFun: string → option fspec. (* SpcPureFun stores fspecs which repeat use *)
+  Context (genv : GEnv.t).
+  Context (u u_apc : univ_id).
+  Context (spc spc_pure spc_pure_fun : string → option fspec). (* spc_pure_fun stores fspecs which repeat use *)
 
   (* SPC Hypothesis *)
-  Hypothesis APCInSpcPure: spc_incl APCA.Spc SpcPure.
-  Hypothesis SpcPureInSpc: spc_sub SpcPure Spc.
-  Hypothesis SpcPureFunInSpcPure: spc_sub SpcPureFun SpcPure.
-  Hypothesis repeatInSpcPure: SpcPure RepeatName.repeat = Some (RepeatAS.repeat_spec SpcPureFun genv). (* to avoid recursive definition of SpcPure *)
+  Context (APCInSpcPure : spc_incl APCA.Spc spc_pure).
+  Context (SpcPureInSpc : spc_sub spc_pure spc).
+  Context (SpcPureFunInSpcPure : spc_sub spc_pure_fun spc_pure).
+  Context (repeatInSpcPure : spc_pure RepeatName.repeat = Some (RepeatAS.repeat_spec spc_pure_fun genv)). (* to avoid recursive definition of SpcPure *)
 
   (* Modules *)
-  Local Definition APCA := (APCA.t u SpcPure Spc).
+  Local Definition APCA := (APCA.t u_apc spc_pure spc).
   Local Definition RepeatI := (RepeatI.t genv).
-  Local Definition RepeatA := (RepeatA.t genv u Spc SpcPureFun).
+  Local Definition RepeatA := (RepeatA.t genv u spc spc_pure_fun).
   Local Definition RepeatIMod := (RepeatI ★ APCA).
   Local Definition RepeatAMod := (RepeatA ★ APCA).
 
   (* IST *)
-  Definition Ist : nat → alist key Any.t → alist key Any.t → iProp :=
+  Definition Ist : nat → alist key Any.t → alist key Any.t → iProp Σ :=
     (λ _ st_src st_tgt, emp%I).
   Local Definition IstFull := (IstProd (IstSB RepeatA.(HMod.scopes) Ist) IstEq).
-
-  (* tactic to simplify meta/precond/postcond for fspecs *)
-  Ltac _fspec_simpl_core := unfold SMod2HMod.meta, SMod2HMod.precond, SMod2HMod.postcond in *; simpl in *.
-  Tactic Notation "fspec_simpl" := _fspec_simpl_core.
-  Tactic Notation "fspec_simpl" constr(p) := try (depdes p); _fspec_simpl_core.
-
-  (* auxiliary fn_has_spec-related lemma *)
-  (* Lemma fn_has_spec_trivial :
-    ∀ Spc fn fsp,
-        Spc fn = Some fsp → fn_has_spec Spc fn fsp.
-  Proof.
-    ii. do 2 (econs; et). by split; r; iIntros; iModIntro.
-  Qed. *)
 
   Lemma simF_repeat : HSim.sim_fun open RepeatAMod RepeatIMod IstFull RepeatName.repeat.
   Proof.
     (* Simulation Start *)
-    init_simF.
+    winit_simF u 0.
 
     (* SRC: handle the precond of repeat *)
-    steps_l. rename q2 into f_sem, q3 into n, q4 into x.
-    iDestruct "ASM" as "%". hss. dup H3. inv H3. steps_l.
+    wsteps_l. rename q2 into f_sem, q3 into n, q4 into x.
+    iDestruct "ASM" as "%". hss. dup H3. inv H3. wsteps_l.
 
     (* TGT: handle input *)
-    steps_r. unfold assume. force_r. steps_r.
+    wsteps_r. unfold assume. wforce_r. wsteps_r.
 
     (* case analysis: n *)
     destruct n as [|n'].
@@ -65,31 +49,31 @@ Module RepeatIA. Section RepeatIA.
     (* CASE: n is 0 *)
     {
       (* TGT: steps tgt *)
-      hss. steps_r.
+      hss. wsteps_r.
 
       (* SRC: unfold APC *)
-      forces_l. iSplit. { iPureIntro. apply SpcPureInSpc. apply APCInSpcPure. unfold APCA.Spc. unseal CRIS. et. }
-      steps_l. forces_l. iSplit; et. inline_l. steps_l. iDestruct "ASM" as "%". hss.
-      steps_l. unfold APC. force_l. steps_l.
+      wforces_l. iSplit. { iPureIntro. apply SpcPureInSpc. apply APCInSpcPure. unfold APCA.Spc. unseal CRIS. et. }
+      wsteps_l. wforces_l. iSplit; et. winline_l. wsteps_l. iDestruct "ASM" as "%". hss.
+      wsteps_l. unfold APC. wforce_l. wsteps_l.
 
       (* SRC: change to skip *)
-      apc_l. steps_l. forces_l. iSplit; et. steps_l. forces_l. iSplit; et.
+      apc_l. wsteps_l. wforces_l. iSplit; et. wsteps_l. wforces_l. iSplit; et.
 
       (* prove the IST *)
-      step. by iSplit.
+      wstep. by iSplit.
     }
 
     (* CASE: n is S n' *)
     {
       (* TGT: load fn from function pointer *)
       destruct (Z_lt_le_dec (S n') 1) eqn:E; try lia.
-      rewrite H2. hss. steps_r.
+      rewrite H2. hss. wsteps_r.
 
       (* SRC: unfold APC *)
-      force_l. iSplit. { iPureIntro. apply SpcPureInSpc. apply APCInSpcPure. unfold APCA.Spc. unseal CRIS. et. }
-      steps_l. fspec_simpl. forces_l. iSplit; et. steps_l.
-      inline_l. fspec_simpl. steps_l. iDestruct "ASM" as "%". hss.
-      steps_l. unfold APC. force_l 2. steps_l.
+      wforce_l. iSplit. { iPureIntro. apply SpcPureInSpc. apply APCInSpcPure. unfold APCA.Spc. unseal CRIS. et. }
+      wsteps_l. wforces_l. iSplit; et. wsteps_l.
+      winline_l. wsteps_l. iDestruct "ASM" as "%". hss.
+      wsteps_l. unfold APC. wforce_l 2. wsteps_l.
 
       (* call apc with fn *)
       apc_call_weaker "IST"; et.
@@ -99,7 +83,7 @@ Module RepeatIA. Section RepeatIA.
       iDestruct "ISTPOST" as "[IST %]". unfold postcond. subst.
 
       (* TGT: steps tgt *)
-      steps_r. hss. steps_r. assert (S n' - 1 = n')%Z as -> by lia.
+      wsteps_r. hss. wsteps_r. assert (S n' - 1 = n')%Z as -> by lia.
 
       (* call apc with repeat *)
       apc_call "IST"; et.
@@ -112,13 +96,13 @@ Module RepeatIA. Section RepeatIA.
       iDestruct "ISTPOST" as "[IST %]". subst.
 
       (* TGT: steps tgt *)
-      steps_r. hss. steps_r.
+      wsteps_r. hss. wsteps_r.
 
       (* SRC: change to skip *)
-      apc_l. steps_l. forces_l. iSplit; et. steps_l. forces_l. iSplit; et.
+      apc_l. wsteps_l. wforces_l. iSplit; et. wsteps_l. wforces_l. iSplit; et.
 
       (* prove the IST *)
-      step. by iSplit.
+      wstep. by iSplit.
     }
     Unshelve. all: et. exact (0↑).
   Qed.
@@ -130,14 +114,17 @@ Module RepeatIA. Section RepeatIA.
       repeat (iSplit; eauto); iPureIntro; ss.
     - apply simF_repeat; eauto.
   Qed.
+End RepeatIA. 
+Section wctxr.
+  Context `{!invG α Σ Γ, !subG Γ Σ, !sinvG Σ Γ α β τ}.
 
-  Theorem correct :
+  Definition wctxr (ge : GEnv.t) (u u_apc : univ_id) (spc spc_pure spc_pure_fun : string → option fspec)
+        (APCInSpcPure : spc_incl APCA.Spc spc_pure)
+        (SpcPureInSpc : spc_sub spc_pure spc)
+        (SpcPureFunInSpcPure : spc_sub spc_pure_fun spc_pure)
+        (repeatInSpcPure: spc_pure RepeatName.repeat = Some (RepeatAS.repeat_spec spc_pure_fun ge)) :
     ctx_refines
-      (RepeatA  ★  APCA, RepeatA.InitCond)
-      ((RepeatI.t genv) ★  APCA, emp%I).
-  Proof.
-    eapply main_adequacy.
-    eapply RepeatIA.sim; et.
-  Qed.
-
-End RepeatIA. End RepeatIA.
+      ((RepeatA.t ge u spc spc_pure_fun) ★ (APCA.t u_apc spc_pure spc), emp%I)
+      ((RepeatI.t ge)                    ★ (APCA.t u_apc spc_pure spc), emp%I).
+  Proof. eapply main_adequacy, sim; eauto. Qed.
+End wctxr. End RepeatIA.
